src/Polara/Optimizations/Basics.lean
@@ -1,0 +1,4 @@
+import Polara.Syntax.Index
+import Polara.Optimizations.ToAinf
+import Polara.Optimizations.ToTm
+import Polara.Optimizations.NbE
