src/Polara/Optimizations/CleanEnv.lean
@@ -1,0 +1,30 @@
+import Polara.Syntax.Index
+import Polara.Optimizations.ToAinf
+
+-- requires topological order
+def Bnds.cleanEnv (res: Bnds): Bnds → Bnds
+| [] => res
+| bnd :: bnds' =>
+  let ⟨⟨_,v⟩,env,prim⟩ := bnd
+  let pars := Bnd.pars bnd
+  let vars := Bnd.vars bnd
+  let defsEnv: List EnvPart := vars.flatMap (λ ⟨_,v⟩ => (v.lookupEnvB res).get!) -- remove duplicates?
+  let env' := env.filter (λ
+    -- an envPart isn't needed if its par isn't directly used or used by a required def
+    | .func _ x => pars.contains ⟨_,x⟩ ∨ defsEnv.contains (.func _ x)
+    | .forc _ i => pars.contains ⟨_,i⟩ ∨ defsEnv.contains (.forc _ i)
+    | .itec _ _ => true -- itec always good to have
+  )
+  Bnds.cleanEnv (res.concat ⟨⟨_,v⟩,env',prim⟩) bnds'
+
+def AINF.cleanEnv: AINF α → AINF α
+| (bnds, ret) => (Bnds.cleanEnv [] bnds, ret)
+
+
+open Ty
+#eval (for' i:10 => (tlitf 1) + (tlitf 1)).toAINF.cleanEnv
+#eval (for' i:10 => (tlitf 1) + i.i2n.n2f).toAINF.cleanEnv
+#eval (for' i:10 => if' i.i2n then (tlitf 0) else (tlitf 1)).toAINF.cleanEnv
+
+-- todo push itec as far back as possible? (loop unswitching)
+#eval (for' i:10 => for' j:10 => if' i.i2n then (tlitf 0) else j.i2n.n2f).toAINF.cleanEnv
