src/Polara/Optimizations/Vectorization.lean
@@ -1,0 +1,47 @@
+import Polara.Optimizations.Basics
+import Polara.Optimizations.CleanEnv
+
+def AINF.vectorize (ainf: AINF α): AINF α :=
+  ainf.flatMapMBnd id (λ bnd => match bnd with
+    | ⟨⟨α,v⟩,env,prim⟩ =>
+      match prim with
+      | .cst2 cst2 a b (α₁:=α') (α₂:=β') (α:=γ') =>
+        match a, b with
+        | .v av, .v bv =>
+          let (envPrefix,restPrefixes) := #[
+            env,
+            av.lookupEnv ainf |>.get!,
+            bv.lookupEnv ainf |>.get!,
+          ].toVector.splitListPrefix
+          let envR := restPrefixes[0]
+          let aER := restPrefixes[1]
+          let bER := restPrefixes[2]
+          match cst2 with
+          | .arithOp (type:=_) op =>
+            match envPrefix with -- todo allow multiple forc
+            | (.forc n i) :: env' => do
+              let ar := (←VParM.var) (α'.array n)
+              let br := (←VParM.var) (β'.array n)
+              let cr := (←VParM.var) (γ'.array n)
+              return [
+                -- env in val
+                ⟨⟨_,ar⟩, (env'.append aER), Prim.bld i a⟩,
+                ⟨⟨_,br⟩, (env'.append bER), Prim.bld i b⟩,
+                -- vec op
+                ⟨⟨_,cr⟩, (env'.append envR), Prim.cst2 (.arithOp op) (.v ar) (.v br)⟩,
+                -- val in vec
+                ⟨⟨_,v ⟩, (env.append envR) , Prim.cst2 (.get) (.v cr) (.p i)⟩
+              ]
+            | _ => pure [bnd]
+          | _ => pure [bnd]
+        | _, _ => pure [bnd]
+      | _ => pure [bnd]
+  )
+
+open Ty
+#eval (for' i:10 => tlitf 1 + tlitf 1).toAINF.cleanEnv.vectorize -- no vecotrization
+#eval (fun' a => for' i:10 => a[[i]] + (tlitf 1)).toAINF.cleanEnv.vectorize -- no vectorize?
+#eval (fun' a: flt.array 10 => for' i:10 => a[[i]] + a[[i]]).toAINF.cleanEnv.vectorize -- vectorize
+#eval (fun' a => for' i:10 => (a[[i]] + a[[i]]) + a[[i]]).toAINF.cleanEnv.vectorize -- vectorize
+
+-- todo vecotrization gets optimized away by .toTm.normVPar
